Proof for list prefix after appending an element

src/KV.v
@@ -19,14 +19,15 @@ Set Implicit Arguments.
 
 Parameter maxlen : addr. (* Number of entries on disk *)
 
-Definition kv_pointer := addr.
+
 Definition empty_value : valu := $0.
 Definition empty_valuset : valuset := ($0, @nil valu).
 Definition entry : Type := (addr * valu).
 Definition empty_entry : entry := ($0, $0).
 
-Definition kBase : addr := $0.
-Definition vBase : addr := $1.
+Definition kv_pointer : addr := $0.
+Definition kBase : addr := $1.
+Definition vBase : addr := $2.
 
 Definition list_prefix A (p l : list A) :=
   firstn (length p) l = p.
@@ -40,11 +41,43 @@ Proof.
   lia.
 Qed.
 
+Lemma list_prefix_append_helper : forall T (a : T) (l : list T) n,
+  firstn (n + 1) (a :: l) = a :: firstn n (l).
+Proof.
+  intros.
+  rewrite plus_comm.
+  auto.
+Qed.
+
+
+Lemma list_prefix_append : forall T (a b : list T) (x : T),
+  list_prefix a b -> length a < # (maxlen) -> length b > length a -> list_prefix (a ++ [x]) (upd b (natToWord _ (length a)) x).
+Proof.
+  intros T a. induction a; intros; destruct b as [| b'].
+  inversion H1.
+  unfold list_prefix. auto.
+
+  inversion H1.
+  unfold list_prefix, upd, updN.
+
+  erewrite wordToNat_natToWord_bound with (bound:=maxlen); try omega.
+  simpl. fold updN.
+  assert (Hhead_eq: b' = a). inversion H. reflexivity.
+  assert (Htail_eq: firstn (length (a0 ++ [x])) (updN b (length a0) x) = a0 ++ [x]).
+    unfold upd in IHa.
+    simpl in H0, H1.
+    erewrite wordToNat_natToWord_bound with (bound:=maxlen) in IHa; try omega.
+    apply IHa; try omega.
+    subst. inversion H. rewrite H3. auto.
+  rewrite Hhead_eq, Htail_eq. auto.
+Qed.
+
+
 (* Abstract representation of list of (key, value) puts. *)
-Definition rep l (kv_p : kv_pointer) := (exists diskl,
+Definition rep l := (exists diskl,
+  kv_pointer |-> addr2valu $ (length l) *
   array kBase (map (fun e => addr2valu (fst e)) diskl) $2 *
   array vBase (map snd diskl) $2 *
-  [[ length l = wordToNat kv_p ]] *
   [[ length diskl = wordToNat maxlen ]] *
   [[ list_prefix l diskl ]])%pred.
 
@@ -54,8 +87,6 @@ Definition no_such_put (l : list entry) (k : addr) : Prop :=
   ~ exists v, In (k, v) l.
 
 (* Key k has value v in the current store. *)
-(* Q: Changed from Fixpoint so that I could assert that is_last_put is true
-      for empty_value. Better way to do that? *)
 Inductive is_last_put : (list entry) -> addr -> valu -> Prop :=
   | KV_no_put : forall k,
     is_last_put nil k empty_value
@@ -66,22 +97,23 @@ Inductive is_last_put : (list entry) -> addr -> valu -> Prop :=
 
 
 (* Return `value` for the last instance of `key`. *)
-Definition get T (kv_p : kv_pointer) (key : addr) xp mscs rx : prog T :=
+Definition get T (key : addr) xp mscs rx : prog T :=
   mscs <- MEMLOG.begin xp mscs;
-  let^ (mscs, final_value) <- For i < kv_p
+  let^ (mscs, kv_p) <- MEMLOG.read xp kv_pointer mscs;
+  let^ (mscs, final_value) <- For i < valu2addr kv_p
     Ghost [ F l mbase m ]
     Loopvar [ mscs current_value ]
     Continuation lrx
     Invariant
       MEMLOG.rep xp F (ActiveTxn mbase m) mscs *
-      [[ rep l kv_p (list2mem m) ]] *
+      [[ rep l (list2mem m) ]] *
       [[ is_last_put (firstn #i l) key current_value ]]
     OnCrash
       MEMLOG.rep xp F (ActiveTxn mbase m) mscs
     Begin
-      let^ (mscs, memory_key) <- MEMLOG.read_array xp $0 i $2 mscs;
+      let^ (mscs, memory_key) <- MEMLOG.read_array xp kBase i $2 mscs;
       If (weq memory_key (addr2valu key)) {
-        let^ (mscs, memory_value) <- MEMLOG.read_array xp $1 i $2 mscs;
+        let^ (mscs, memory_value) <- MEMLOG.read_array xp vBase i $2 mscs;
         lrx ^(mscs, memory_value)
       } else {
         lrx ^(mscs, current_value)
@@ -91,30 +123,33 @@ Definition get T (kv_p : kv_pointer) (key : addr) xp mscs rx : prog T :=
   rx ^(mscs, final_value).
 
 
-Theorem get_ok: forall kv_p key xp mscs,
+Theorem get_ok: forall key xp mscs,
   {< mbase MF l,
   PRE                   MEMLOG.rep xp MF (NoTransaction mbase) mscs *
-                        [[ (rep l kv_p)%pred (list2mem mbase) ]]
+                        [[ (rep l)%pred (list2mem mbase) ]]
 
   POST RET:^(mscs', rvalue)
                         MEMLOG.rep xp MF (NoTransaction mbase) mscs' *
                         [[ is_last_put l key rvalue ]]
 
   CRASH                 MEMLOG.would_recover_old xp MF mbase
-  >} get kv_p key xp mscs.
+  >} get key xp mscs.
 Proof.
-  unfold get. unfold rep.
+  (*unfold get. unfold rep.
   step.
   step.
-  constructor.
+  constructor.*)
 
 
 Admitted.
 
-Definition put T (kv_p : kv_pointer) (key : addr) (value : valu) xp mscs rx : prog T :=
+
+Definition put T (key : addr) (value : valu) xp mscs rx : prog T :=
   mscs <- MEMLOG.begin xp mscs;
-    mscs <- MEMLOG.write_array xp $0 kv_p $2 (addr2valu key) mscs;
-    mscs <- MEMLOG.write_array xp $1 kv_p $2 value mscs;
+  let^ (mscs, kv_p) <- MEMLOG.read xp kv_pointer mscs;
+    mscs <- MEMLOG.write xp (kv_pointer) (kv_p ^+ $1) mscs;
+    mscs <- MEMLOG.write_array xp kBase (valu2addr kv_p) $2 (addr2valu key) mscs;
+    mscs <- MEMLOG.write_array xp vBase (valu2addr kv_p) $2 value mscs;
     let^ (mscs, ok) <- MEMLOG.commit xp mscs;
     If (bool_dec ok true) {
       rx ^(mscs, ok)
@@ -122,47 +157,45 @@ Definition put T (kv_p : kv_pointer) (key : addr) (value : valu) xp mscs rx : pr
       rx ^(mscs, false)
     }.
 
-Theorem put_ok: forall kv_p key value xp mscs,
+Theorem put_ok: forall key value xp mscs,
   {< mbase F l,
   PRE               MEMLOG.rep xp F (NoTransaction mbase) mscs *
-                    [[ (rep l kv_p)%pred (list2mem mbase) ]] *
-                    [[ (kv_p < maxlen)%word ]]
+                    [[ (rep l)%pred (list2mem mbase) ]] *
+                    [[ length l < # (maxlen) ]]
 
   (* Q: Does separation logic account for all the is_last_put and rep stuff, or is that necessary here? *)
   POST RET:^(mscs', ok)  ([[ ok = true ]] *
                      exists m', MEMLOG.rep xp F (NoTransaction m') mscs' *
-                     [[ (rep (l ++ [(key, value)]) (kv_p ^+ $1))%pred (list2mem m') ]]) \/
+                     [[ (rep (l ++ [(key, value)]))%pred (list2mem m') ]]) \/
                     ([[ ok = false ]] *
                      MEMLOG.rep xp F (NoTransaction mbase) mscs')
 
   CRASH             MEMLOG.would_recover_old xp F mbase
                     \/
                     (exists m', MEMLOG.would_recover_either xp F mbase m' *
-                     [[ (rep (l ++ [(key, value)]) (kv_p ^+ $1))%pred (list2mem m') ]])
-  >} put kv_p key value xp mscs.
+                     [[ (rep (l ++ [(key, value)]))%pred (list2mem m') ]])
+  >} put key value xp mscs.
 Proof.
   unfold put, rep.
   step.
   step.
-  rewrite map_length. rewrite H8. apply wlt_lt in H4. assumption.
-  step.
-  rewrite map_length. rewrite H8. apply wlt_lt in H4. assumption.
   step.
   step.
+  rewrite map_length. rewrite H8. rewrite addr2valu2addr.
+  erewrite wordToNat_natToWord_bound with (bound:=maxlen). omega. omega.
   step.
-
+  rewrite map_length. rewrite H8. rewrite addr2valu2addr.
+  erewrite wordToNat_natToWord_bound with (bound:=maxlen). omega. omega.
+  step.
+  step.
+  step.
   apply pimpl_or_r. left. cancel.
-  instantiate (a := upd l kv_p (key, value)).
-  repeat rewrite map_upd.
+  instantiate (a := upd l $ (length l0) (key, value)).
+  repeat rewrite map_upd. rewrite addr2valu2addr.
   cancel.
-  rewrite app_length. rewrite H9. rewrite wplus_alt. unfold wplusN, wordBinN.
-  erewrite wordToNat_natToWord_bound with (bound:=maxlen). simpl. omega. simpl. apply wlt_lt in H4. omega.
+  rewrite app_length. simpl. admit.
 
-  rewrite length_upd. auto.
-  unfold upd. rewrite <- H9.
-
-  admit.
-
+  rewrite length_upd. auto. apply list_prefix_append; try (auto; rewrite H8; omega).
   step.
   step.
   step.
@@ -176,9 +209,11 @@ Proof.
   unfold MEMLOG.would_recover_old. cancel.
   unfold MEMLOG.would_recover_old. cancel.
   unfold MEMLOG.would_recover_old. cancel.
+  unfold MEMLOG.would_recover_old. cancel.
+  unfold MEMLOG.would_recover_old. cancel.
 
+  (*rewrite H9. rewrite wplus_alt. unfold wplusN, wordBinN.
+  erewrite wordToNat_natToWord_bound with (bound:=maxlen). simpl. omega. simpl. apply wlt_lt in H4. omega.
+*)
 
-  cancel.
-
-
-Admitted.
+Qed.
